Work on getting the translator working again.
It fails with a completely opaque error message.

print_ast/Print_astTerminationScript.sml
@@ -33,10 +33,10 @@ val _ = register "join_trees" join_trees_def join_trees_ind;
 
 val (pat_to_tok_tree_def, pat_to_tok_tree_ind) =
   tprove_no_defn ((pat_to_tok_tree_def, pat_to_tok_tree_ind),
-  wf_rel_tac `measure (\x. pat_size (\x.0) x)` >>
+  wf_rel_tac `measure pat_size` >>
   rw [] >|
   [decide_tac,
-   induct_on `v8` >>
+   induct_on `v7` >>
        rw [] >>
        fs [pat_size_def] >>
        decide_tac]);
@@ -44,14 +44,14 @@ val _ = register "pat_to_tok_tree" pat_to_tok_tree_def pat_to_tok_tree_ind;
 
 val (exp_to_tok_tree_def, exp_to_tok_tree_ind) =
   tprove_no_defn ((exp_to_tok_tree_def, exp_to_tok_tree_ind),
-  wf_rel_tac `measure (\x. case x of INL (_,e) => exp_size (\x.0) e
-                                   | INR (INL (_,p,e)) => exp_size (\x.0) e + 1
-                                   | INR (INR (_,v1,topt1,v2,topt2,e)) => exp_size (\x.0) e + 1)` >>
+  wf_rel_tac `measure (\x. case x of INL (_,e) => exp_size e
+                                   | INR (INL (_,p,e)) => exp_size e + 1
+                                   | INR (INR (_,topt1,topt2,e)) => exp_size e + 1)` >>
   rw [] >>
   TRY (induct_on `funs`) >>
   TRY (induct_on `pes`) >>
   TRY (induct_on `es`) >>
-  TRY (induct_on `v49`) >>
+  TRY (induct_on `v43`) >>
   rw [exp_size_def] >>
   fs [exp_size_def] >>
   rw [exp_size_def] >>
